Hom2 -> Hom

Kura/Comp/Brook.lean
@@ -7,5 +7,20 @@ variable {α α' β β' : Type*} {G G' H H' : Graph α β} {x y z u v : α} {e f
 
 namespace Graph
 
+
+def IsCycleGraph (G : Graph α β) : Prop := sorry
+def IsCompleteGraph (G : Graph α β) : Prop := sorry
+
 theorem brooks_theorem (G : Graph α β) [G.Simple] [hV : Finite V(G)] [hE : Finite E(G)]
-    
+    [DecidableRel (G.Adj · ·)] (hG : G.Connected) :
+    G.IsCycleGraph ∨ G.IsCompleteGraph ∨ G.ChromaticNumber ≤ Δ(G) := by
+  rw [Classical.or_iff_not_imp_left, Classical.or_iff_not_imp_left]
+  rintro hC hK
+
+  -- Block decomposition
+  -- obtain h2conn | h2nconn := em (G.NConnected 2)
+
+  obtain hnonreg | hreg := (em (G.regular)).symm
+  · obtain ⟨v, hv, hvdeg⟩ : ∃ x ∈ V(G), G.degree x < Δ(G) := sorry -- not regular
+
+  sorry
